# Precalc Practice

## 3. Conic Sections

### 3.07: Hyperbolas

#### Practice: General Form of a Hyperbola

1. What is the general form of the hyperbola whose equation is:

```
(x+3)^2 / 36 - (y - 1)^2/9 = 1
```

Show work:

```
*36

(x+3)^2 - 4*(y-1)^2 = 36

x^2 + 6x + 9 - 4 * (y^2 - 2y + 1) = 36

x^2 + 6x + 9 - 4y^2 + 8y - 4 = 36

x^2 - 4y^2 + 6x + 8y + 5 = 36

-36

x^2 - 4y^2 + 6x + 8y - 31 = 0
```

![image_1](3%20-%20Conic%20Sections/3-07%20-%20Hyperbolas/image_1.png)

2. What is the general form of the hyperbola whose equation is

```
x^2 / 4 - (y + 7)^2 / 25 = 1
```

Show work:

```
*100

25x^2 - 4 * (y + 7)^2 = 100

25x^2 - 4 * (y^2 + 14y + 49) = 100

25x^2 - 4y^2 - 56y - 196 = 100

-100

25x^2 - 4y^2 - 56y - 296 = 0
```

![image_2](3%20-%20Conic%20Sections/3-07%20-%20Hyperbolas/image_2.png)

3. What is the standard form of the hyperbola whose equation is

```
5x^2 - 2y^2 - 20x - 12y - 18 = 0
```

Show work:

```
5x^2 - 2y^2 - 20x - 12y - 18 = 0

+18

5x^2 - 2y^2 - 20x - 12y = 18

5x^2 - 20x - 2y^2 - 12y = 18

5(x^2 - 4x + a) - 2(y^2 +6y + b) = 18

5(x^2 - 4x + a) - 2(y^2 +6y + b) = 18 + 5(a^2) - 2(b^2)

a * 2 = -4

a = -2

b * 2 = 6

b = 3

5(x - 2)^2 - 2(y + 3)^2 = 18 + 5(4) - 2(9)

5(x - 2)^2 - 2(y - 3)^2 = 18 + 20 - 18

5(x - 2)^2 - 2(y - 3)^2 = 20

/ 20

(x - 2)^2 / 4 - (y - 3)^2 / 10 = 1

```

![image_3](3%20-%20Conic%20Sections/3-07%20-%20Hyperbolas/image_3.png)

4. What is the standard form of the hyperbola whose equation is

```
-2x^2 + y^2 + 8x + 10y + 9 = 0
```

Show work:

```
-2x^2 + y^2 + 8x + 10y + 9 = 0

-9

-2x^2 + y^2 + 8x + 10y = -9

-2x^2 + 8x + y^2 + 10y = -9

-2(x^2 - 4x + a) + (y^2 + 10y + b) = -9

-2(x^2 - 4x + a) + (y^2 + 10y + b) = -9 - 2(a^2) + 1(b^2)

a * 2 = -4

a = -2

b * 2 = 10

b = 5

-2(x - 2)^2 + (y + 5)^2 = -9 -2(4) + 1(25)

-2(x - 2)^2 + (y + 5)^2 = -9 -8 + 25

-2(x - 2)^2 + (y + 5)^2 = 8

/ 8

(x - 2)^2 / -4 + (y + 5)^2 / 8 = 1

(y + 5)^2 / 8 - (x - 2)^2 / 4 = 1
```

![image_4](3%20-%20Conic%20Sections/3-07%20-%20Hyperbolas/image_4.png)
